Typing.thy
@@ -182,6 +182,35 @@ proof -
   then show "\<Delta> \<turnstile> \<Gamma>' @ \<Gamma> \<longrightarrow> P \<Delta> \<Gamma>'" and "\<Gamma>' @ \<Gamma> , \<Delta> \<turnstile>\<^sub>t\<^sub>y \<tau> : k2 \<longrightarrow> Q \<Gamma>' \<Delta> \<tau> k2" by simp_all
 qed
 
+thm term_alt_list_alt.inducts(2)
+
+lemma alts_induct[consumes 1, case_names MatchCtor]:
+  assumes "\<forall>alt |\<in>| set_alts alts. (\<exists>K tys vals e' cty ks args \<Gamma>'.
+                alt = MatchCtor K tys vals e' \<and>
+                AxCtor K cty \<in> set \<Delta> \<and> ctor_type cty = Some (T, ks) \<and>
+                subst_ctor cty \<sigma>s = Some args \<and>
+                \<Gamma>' = zip_with BVar vals args @ zip_with BTyVar tys ks @ \<Gamma> \<and>
+                \<Gamma>' , \<Delta> \<turnstile> e' : \<tau> \<and> P \<Gamma>' e'
+              )"
+  and "\<And>K tys vals e' cty ks args. \<lbrakk> AxCtor K cty \<in> set \<Delta> ; ctor_type cty = Some (T, ks) ; subst_ctor cty \<sigma>s = Some args ;
+        zip_with BVar vals args @ zip_with BTyVar tys ks @ \<Gamma> , \<Delta> \<turnstile> e' : \<tau> ; P (zip_with BVar vals args @ zip_with BTyVar tys ks @ \<Gamma>) e' \<rbrakk> \<Longrightarrow> Q \<Gamma> (MatchCtor K tys vals e')"
+shows "\<forall>alt |\<in>| set_alts alts. Q \<Gamma> alt"
+proof -
+  let ?W = "\<lambda>alt. (\<exists>K tys vals e' cty ks args \<Gamma>'.
+                alt = MatchCtor K tys vals e' \<and>
+                AxCtor K cty \<in> set \<Delta> \<and> ctor_type cty = Some (T, ks) \<and>
+                subst_ctor cty \<sigma>s = Some args \<and>
+                \<Gamma>' = zip_with BVar vals args @ zip_with BTyVar tys ks @ \<Gamma> \<and>
+                \<Gamma>' , \<Delta> \<turnstile> e' : \<tau> \<and> P \<Gamma>' e')"
+  show ?thesis
+  using assms(1) proof (induction alts rule: term_alt_list_alt.inducts(2)[of "\<lambda>_. True" _ "\<lambda>alt. ?W alt \<longrightarrow> Q \<Gamma> alt"])
+  next
+    case (MatchCtor K tys vals e')
+    then show ?case using assms(2) apply auto
+      by (metis term_alt_list_alt.eq_iff(11))
+  qed simp_all
+qed
+
 (* context validity *)
 lemma context_valid_ty: "\<Gamma> , \<Delta> \<turnstile>\<^sub>t\<^sub>y \<tau> : \<kappa> \<Longrightarrow> \<Delta> \<turnstile> \<Gamma>"
   by (induction \<Gamma> \<Delta> \<tau> \<kappa> rule: Ty_induct) auto
@@ -228,6 +257,345 @@ proof goal_cases
 qed auto
 
 
+lemma context_cons_valid[elim]: "(\<Delta>::\<Delta>) \<turnstile> bndr # \<Gamma> \<Longrightarrow> (\<Delta> \<turnstile> \<Gamma> \<Longrightarrow> P) \<Longrightarrow> P"
+  by (cases rule: Ctx.cases) (auto simp: context_valid(1))
+
+lemma axioms_split_valid: "\<turnstile> \<Delta>' @ \<Delta> \<Longrightarrow> \<turnstile> \<Delta>"
+proof (induction \<Delta>')
+  case (Cons a \<Delta>')
+  then show ?case using axioms_valid(2) by (cases a rule: axiom.exhaust) auto
+qed simp
+
+
+lemma isin_same_kind: "\<lbrakk> BTyVar a k1 \<in> (\<Gamma>' @ BTyVar a k2 # \<Gamma>) ; \<Delta> \<turnstile> \<Gamma>' @ BTyVar a k2 # \<Gamma> \<rbrakk> \<Longrightarrow> k1 = k2"
+proof (induction \<Gamma>')
+  case (Cons bndr \<Gamma>')
+  then show ?case by (cases rule: Ctx.cases[OF Cons(3)]) (auto split: if_splits simp: fresh_Cons fresh_append fresh_at_base(2))
+qed auto
+
+lemma isin_same_type: "\<lbrakk> BVar x \<tau> \<in> (\<Gamma>' @ BVar x \<tau>2 # \<Gamma>) ; \<Delta> \<turnstile> \<Gamma>' @ BVar x \<tau>2 # \<Gamma> \<rbrakk> \<Longrightarrow> \<tau> = \<tau>2"
+proof (induction \<Gamma>')
+  case (Cons a \<Gamma>')
+  then show ?case by (cases rule: Ctx.cases[OF Cons(3)]) (auto split: if_splits simp: fresh_Cons fresh_append fresh_at_base)
+qed auto
+lemmas isin_same = isin_same_kind isin_same_type
+
+lemma isin_subset:
+  fixes \<Gamma>::"\<Gamma>"
+  assumes "\<Delta> \<turnstile> \<Gamma>' @ \<Gamma>"
+  shows "bndr \<in> \<Gamma> \<longrightarrow> bndr \<in> (\<Gamma>' @ \<Gamma>)"
+proof
+  assume "bndr \<in> \<Gamma>"
+  then show "bndr \<in> (\<Gamma>' @ \<Gamma>)"
+  using assms proof (induction \<Gamma>' arbitrary: \<Gamma>)
+    case (Cons b \<Gamma>2)
+    have 1: "\<Delta> \<turnstile> \<Gamma>2 @ \<Gamma>" using Cons(3) by auto
+    have 2: "bndr \<in> (\<Gamma>2 @ \<Gamma>)" by (rule Cons(1)[OF Cons(2) 1])
+    show ?case
+    proof (cases b rule: binder.exhaust)
+      case (BVar x \<tau>)
+      then have "atom x \<sharp> (\<Gamma>2 @ \<Gamma>)" using Cons by auto
+      then show ?thesis using 2 BVar fresh_not_isin_var by (cases bndr rule: binder.exhaust) auto
+    next
+      case (BTyVar a k)
+      then have "atom a \<sharp> (\<Gamma>2 @ \<Gamma>)" using Cons by auto
+      then show ?thesis using 2 BTyVar fresh_not_isin_tyvar by (cases bndr rule: binder.exhaust) auto
+    qed
+  qed auto
+qed
+
+lemma weaken_isin: "\<lbrakk> bndr \<in> (\<Gamma> @ \<Gamma>') ; \<Delta> \<turnstile> \<Gamma> @ xs @ \<Gamma>' \<rbrakk> \<Longrightarrow> bndr \<in> (\<Gamma> @ xs @ \<Gamma>')"
+proof (induction \<Gamma> arbitrary: bndr \<Gamma>' xs)
+  case Nil
+  then show ?case by (cases bndr rule: binder.exhaust) (auto simp: isin_subset)
+next
+  case (Cons b \<Gamma>)
+  have 1: "\<Delta> \<turnstile> \<Gamma> @ xs @ \<Gamma>'" using Cons(3) Ctx.cases by auto
+  then show ?case
+  proof (cases b rule: binder.exhaust)
+    case (BVar x \<tau>)
+    then show ?thesis using 1 Cons by (cases bndr rule: binder.exhaust) auto
+  next
+    case (BTyVar a k)
+    then show ?thesis using 1 Cons by (cases bndr rule: binder.exhaust) auto
+  qed
+qed
+
+lemma Ty_Forall_Inv:
+  assumes a: "\<Gamma> , \<Delta> \<turnstile>\<^sub>t\<^sub>y (\<forall>a:k. \<sigma>) : \<tau>" and b: "atom a \<sharp> \<Gamma>"
+  shows "BTyVar a k # \<Gamma> , \<Delta> \<turnstile>\<^sub>t\<^sub>y \<sigma> : \<star> \<and> \<tau> = \<star>"
+proof (cases rule: Ty.cases[OF a])
+  case (5 a' k' \<Gamma>' \<Delta>' \<sigma>')
+  then have 1: "(BTyVar a' k # \<Gamma>) , \<Delta> \<turnstile>\<^sub>t\<^sub>y \<sigma>' : \<star>" by simp
+  have valid: "\<turnstile> \<Delta>" by (rule axioms_valid(2)[OF 1])
+  have "(a' \<leftrightarrow> a) \<bullet> \<sigma>' = \<sigma>" using Abs_rename_body[of a' \<sigma>' a \<sigma>] 5(3) by auto
+  then have 2: "((a' \<leftrightarrow> a) \<bullet> (BTyVar a' k # \<Gamma>)) , \<Delta> \<turnstile>\<^sub>t\<^sub>y \<sigma> : \<star>" using Ty.eqvt[OF 1, of "(a' \<leftrightarrow> a)"] valid by auto
+  have 3: "((a' \<leftrightarrow> a) \<bullet> (BTyVar a' k # \<Gamma>)) = BTyVar a k # ((a' \<leftrightarrow> a) \<bullet> \<Gamma>)" using Cons_eqvt flip_fresh_fresh by force
+  have 4: "(a' \<leftrightarrow> a) \<bullet> \<Gamma> = \<Gamma>" by (metis 5(1,5) CtxE(1) b context_valid_ty flip_def swap_fresh_fresh)
+  show ?thesis using 2 3 4 5(4) by argo
+qed simp_all
+
+lemma weaken_ty: "\<lbrakk> \<Gamma> @ \<Gamma>' , \<Delta>  \<turnstile>\<^sub>t\<^sub>y \<tau> : k ; \<Delta> \<turnstile> \<Gamma> @ xs @ \<Gamma>' \<rbrakk> \<Longrightarrow> \<Gamma> @ xs @ \<Gamma>' , \<Delta> \<turnstile>\<^sub>t\<^sub>y \<tau> : k"
+proof (nominal_induct \<tau> avoiding: \<Gamma> \<Gamma>' xs k rule: \<tau>.strong_induct)
+  case (TyVar x)
+  have 1: "BTyVar x k \<in> (\<Gamma> @ \<Gamma>')" by (cases rule: Ty.cases[OF TyVar(1)]) auto
+  show ?case by (rule Ty_Var[OF TyVar(2) weaken_isin[OF 1 TyVar(2)]])
+next
+  case (TyData T)
+  then have "AxData T k \<in> set \<Delta>" by blast
+  then show ?case by (rule Ty_Data[OF TyData(2)])
+next
+  case TyArrow
+  then have "k = (\<star> \<rightarrow> \<star> \<rightarrow> \<star>)" by blast
+  then show ?case using Ty_Arrow[OF TyArrow(2)] by argo
+next
+  case (TyApp \<tau>1 \<tau>2)
+  then obtain k1 where P: "\<Gamma> @ \<Gamma>' , \<Delta> \<turnstile>\<^sub>t\<^sub>y \<tau>1 : k1 \<rightarrow> k" "\<Gamma> @ \<Gamma>' , \<Delta> \<turnstile>\<^sub>t\<^sub>y \<tau>2 : k1" by blast
+  have 2: "\<Gamma> @ xs @ \<Gamma>' , \<Delta> \<turnstile>\<^sub>t\<^sub>y \<tau>1 : k1 \<rightarrow> k" by (rule TyApp(1)[OF P(1) TyApp(4)])
+  have 3: "\<Gamma> @ xs @ \<Gamma>' , \<Delta> \<turnstile>\<^sub>t\<^sub>y \<tau>2 : k1" by (rule TyApp(2)[OF P(2) TyApp(4)])
+  show ?case by (rule Ty_App[OF 2 3])
+next
+  case (TyForall a k1 \<sigma>)
+  have P: "(BTyVar a k1 # \<Gamma>) @ \<Gamma>' , \<Delta> \<turnstile>\<^sub>t\<^sub>y \<sigma> : \<star>" "k = \<star>" using Ty_Forall_Inv[OF TyForall(6)] TyForall(1,2) fresh_append by auto
+  have 1: "atom a \<sharp> \<Gamma> @ xs @ \<Gamma>'" using TyForall(1-3) fresh_append by blast
+  have 2: "\<Delta> \<turnstile> (BTyVar a k1 # \<Gamma>) @ xs @ \<Gamma>'" using Ctx_TyVar[OF TyForall(7) 1] by simp
+  have 3: "BTyVar a k1 # \<Gamma> @ xs @ \<Gamma>' , \<Delta> \<turnstile>\<^sub>t\<^sub>y \<sigma> : \<star>" using TyForall(5)[OF P(1) 2] by simp
+  show ?case using Ty_Forall[OF 3] P(2) by simp
+qed
+
+lemma isin_subst_tyvar: "\<lbrakk> BTyVar a k \<in> (\<Gamma>' @ BTyVar b k2 # \<Gamma>) ; \<Delta> \<turnstile> \<Gamma>' @ BTyVar b k2 # \<Gamma> ; a \<noteq> b \<rbrakk> \<Longrightarrow> BTyVar a k \<in> (\<Gamma>'[\<sigma>/b] @ \<Gamma>)"
+proof (induction \<Gamma>')
+  case (Cons bndr \<Gamma>')
+  then show ?case
+  proof (cases rule: Ctx.cases[OF Cons(3)])
+    case (2 \<Gamma>2 c k3)
+    then have "BTyVar a k = bndr \<or> BTyVar a k \<in> (\<Gamma>' @ BTyVar b k2 # \<Gamma>)" by (metis Cons.prems(1) Cons_eq_append_conv isin.simps(5) list.inject)
+    then show ?thesis
+    proof
+      assume a: "BTyVar a k = bndr"
+      then show ?thesis using 2 Cons by auto
+    next
+      assume "BTyVar a k \<in> (\<Gamma>' @ BTyVar b k2 # \<Gamma>)"
+      then show ?thesis using 2 Cons fresh_not_isin_tyvar by auto
+    qed
+  next
+    case (3 \<Gamma> \<tau> x)
+    then show ?thesis using Cons by auto
+  qed simp
+qed simp
+
+lemma context_valid_append: "\<Delta>::\<Delta> \<turnstile> \<Gamma>' @ \<Gamma> \<Longrightarrow> \<Delta> \<turnstile> \<Gamma>"
+proof (induction \<Gamma>')
+  case (Cons a \<Gamma>')
+  then show ?case using context_valid(1) by (cases a rule: binder.exhaust) auto
+qed auto
+
+lemma axioms_regularity: "\<turnstile> \<Delta>' @ AxCtor D \<tau> # \<Delta> \<Longrightarrow> [] , \<Delta> \<turnstile>\<^sub>t\<^sub>y \<tau> : \<star>"
+  using Ax_Ctor axioms_split_valid by (induction \<Delta>) blast+
+
+lemma context_regularity: "\<Delta> \<turnstile> \<Gamma>' @ BVar x \<tau> # \<Gamma> \<Longrightarrow> \<Gamma> , \<Delta> \<turnstile>\<^sub>t\<^sub>y \<tau> : \<star>"
+  using Ctx_Var context_valid_append by (induction \<Gamma>) blast+
+
+lemma type_substitution_aux:
+  assumes "\<Gamma> , \<Delta> \<turnstile>\<^sub>t\<^sub>y \<sigma> : k"
+  shows "(\<Delta> \<turnstile> (\<Gamma>' @ BTyVar a k # \<Gamma>) \<longrightarrow> \<Delta> \<turnstile> (subst_context \<Gamma>' \<sigma> a @ \<Gamma>))"
+    and "(\<Gamma>' @ BTyVar a k # \<Gamma> , \<Delta> \<turnstile>\<^sub>t\<^sub>y \<tau> : k2 \<longrightarrow> subst_context \<Gamma>' \<sigma> a @ \<Gamma> , \<Delta> \<turnstile>\<^sub>t\<^sub>y subst_type \<tau> \<sigma> a : k2)"
+proof (induction rule: Ctx_Ty_induct_split)
+  case Ctx_Empty
+  then show ?case using context_valid(1)[OF assms] by simp
+next
+  case (Ctx_TyVar \<Gamma>' b k2)
+  then have "atom b \<sharp> \<sigma>" using assms fresh_Cons fresh_append fresh_in_context_ty by blast
+  then have 1: "atom b \<sharp> \<Gamma>'[\<sigma>/a] @ \<Gamma>" by (meson Ctx_TyVar(3) fresh_Cons fresh_append fresh_subst_context_tyvar)
+  show ?case using Ax_Ctx_Ty.Ctx_TyVar[OF Ctx_TyVar(2) 1] assms by auto
+next
+  case (Ctx_Var \<Gamma>' \<tau> x)
+  have 1: "atom x \<sharp> \<Gamma>'[\<sigma>/a] @ \<Gamma>" by (meson Ctx_Var(3) fresh_Cons fresh_append fresh_subst_context_var)
+  show ?case using Ax_Ctx_Ty.Ctx_Var[OF Ctx_Var(2) 1] by simp
+next
+  case (Ty_Var \<Gamma>' b k2)
+  then show ?case
+    proof (cases "b = a")
+    case True
+    then have "k = k2" using isin_same(1) Ty_Var by blast
+    then have "\<Gamma> , \<Delta> \<turnstile>\<^sub>t\<^sub>y (TyVar b)[\<sigma>/a] : k2" using True assms(1) by simp
+    then show ?thesis using weaken_ty[of "[]"] Ty_Var(2) by auto
+  next
+    case False
+    have 1: "BTyVar b k2 \<in> (\<Gamma>'[\<sigma>/a] @ \<Gamma>)" by (rule isin_subst_tyvar[OF Ty_Var(3,1) False])
+    show ?thesis using Ax_Ctx_Ty.Ty_Var[OF Ty_Var(2) 1] False by simp
+  qed
+next
+  case (Ty_Forall \<Gamma>' b k2 \<sigma>')
+  have 1: "a \<noteq> b" by (metis CtxE(1) Ty_Forall(1) binder.fresh(2) context_valid_ty fresh_Cons fresh_append fresh_at_base(2))
+  then have 2: "BTyVar b k2 # \<Gamma>'[\<sigma>/a] @ \<Gamma> , \<Delta> \<turnstile>\<^sub>t\<^sub>y \<sigma>'[\<sigma>/a] : \<star>" using Ty_Forall(2) by simp
+  show "\<Gamma>'[\<sigma>/a] @ \<Gamma> , \<Delta> \<turnstile>\<^sub>t\<^sub>y (\<forall> b : k2 . \<sigma>')[\<sigma>/a] : \<star>" using Ax_Ctx_Ty.Ty_Forall[OF 2]
+    by (metis "1" "2" CtxE(1) assms atom_eq_iff context_valid_ty fresh_Pair fresh_append fresh_at_base(2) fresh_in_context_ty subst_type.simps(5))
+qed (auto intro: Ty_intros)
+corollary type_substitution_context: "\<lbrakk> \<Delta> \<turnstile> \<Gamma>' @ BTyVar a k # \<Gamma> ; \<Gamma> , \<Delta> \<turnstile>\<^sub>t\<^sub>y \<sigma> : k \<rbrakk> \<Longrightarrow> \<Delta> \<turnstile> \<Gamma>'[\<sigma>/a] @ \<Gamma>"
+  using type_substitution_aux by blast
+corollary type_substitution_ty: "\<lbrakk> \<Gamma>' @ BTyVar a k # \<Gamma> , \<Delta> \<turnstile>\<^sub>t\<^sub>y \<tau> : k2 ; \<Gamma> , \<Delta> \<turnstile>\<^sub>t\<^sub>y \<sigma> : k \<rbrakk> \<Longrightarrow> \<Gamma>'[\<sigma>/a] @ \<Gamma> , \<Delta> \<turnstile>\<^sub>t\<^sub>y \<tau>[\<sigma>/a] : k2"
+  using type_substitution_aux by blast
+
+lemma var_strengthen_aux:
+  shows "\<Delta> \<turnstile> \<Gamma>' @ BVar x \<tau> # \<Gamma> \<longrightarrow> \<Delta> \<turnstile> \<Gamma>' @ \<Gamma>"
+  and "\<Gamma>' @ BVar x \<tau> # \<Gamma> , \<Delta> \<turnstile>\<^sub>t\<^sub>y \<sigma> : k \<longrightarrow> \<Gamma>' @ \<Gamma> , \<Delta> \<turnstile>\<^sub>t\<^sub>y \<sigma> : k"
+proof (induction rule: Ctx_Ty_induct_split)
+  case Ctx_Empty
+  then show ?case using context_valid(1) by auto
+next
+  case (Ctx_TyVar \<Gamma>' b k2)
+  then show ?case by (metis Ctx.simps append_Cons fresh_Cons fresh_append)
+next
+  case (Ctx_Var \<Gamma>' \<tau> x)
+  then have "atom x \<sharp> \<Gamma>' @ \<Gamma>" using fresh_append fresh_Cons by blast
+  then show ?case using Ctx_intros(3)[OF Ctx_Var(2)] by simp
+next
+  case (Ty_Var \<Gamma>' b k2)
+  then have "BTyVar b k2 \<in> (\<Gamma>' @ \<Gamma>)" using strengthen_isin_tyvar by simp
+  then show ?case by (rule Ty_intros(1)[OF Ty_Var(2)])
+qed (auto intro: Ty_intros)
+lemma var_strengthen_context: "\<Delta> \<turnstile> \<Gamma>' @ BVar x \<tau> # \<Gamma> \<Longrightarrow> \<Delta> \<turnstile> \<Gamma>' @ \<Gamma>"
+  using var_strengthen_aux by simp
+lemma var_strengthen_ty: "\<Gamma>' @ BVar x \<tau> # \<Gamma> , \<Delta> \<turnstile>\<^sub>t\<^sub>y \<sigma> : k \<Longrightarrow> \<Gamma>' @ \<Gamma> , \<Delta> \<turnstile>\<^sub>t\<^sub>y \<sigma> : k"
+  using var_strengthen_aux by simp
+lemmas strengthen = var_strengthen_context var_strengthen_ty
+
+lemma axiom_isin_split: "\<lbrakk> b \<in> set \<Delta> ; \<turnstile> \<Delta> \<rbrakk> \<Longrightarrow> \<exists>\<Delta>1 \<Delta>2. \<Delta> = \<Delta>1 @ b # \<Delta>2"
+proof (induction \<Delta>)
+  case (Cons a \<Delta>)
+  then show ?case
+  proof (cases "a = b")
+    case True
+    then show ?thesis by blast
+  next
+    case False
+    then show ?thesis by (meson Cons.prems(1) split_list)
+  qed
+qed simp
+
+lemma weaken_axioms_ty: "\<lbrakk> \<Gamma> , \<Delta>' @ \<Delta> \<turnstile>\<^sub>t\<^sub>y \<tau> : k ; \<Delta>' @ xs @ \<Delta> \<turnstile> \<Gamma> \<rbrakk> \<Longrightarrow> \<Gamma> ,  \<Delta>' @ xs @ \<Delta> \<turnstile>\<^sub>t\<^sub>y \<tau> : k"
+proof (nominal_induct \<tau> avoiding: \<Delta> \<Delta>' k xs \<Gamma> rule: \<tau>.strong_induct)
+  case (TyApp \<tau>1 \<tau>2)
+  then show ?case using Ty_App by blast
+next
+  case (TyForall a k1 \<sigma>)
+  have P: "BTyVar a k1 # \<Gamma> , \<Delta>' @ \<Delta> \<turnstile>\<^sub>t\<^sub>y \<sigma> : \<star>" "k = \<star>" using Ty_Forall_Inv[OF TyForall(7,5)] by auto
+  have 1: "BTyVar a k1 # \<Gamma> , \<Delta>' @ xs @ \<Delta> \<turnstile>\<^sub>t\<^sub>y \<sigma> : \<star>" by (rule TyForall(6)[OF P(1) Ctx_TyVar[OF TyForall(8,5)]])
+  show ?case using Ty_Forall[OF 1] P(2) by argo
+qed (auto intro: Ty_intros)
+lemmas weaken = weaken_isin weaken_ty weaken_axioms_ty
+
+lemma typing_regularity: "\<Gamma> , \<Delta> \<turnstile> e : \<tau> \<Longrightarrow> \<Gamma> , \<Delta> \<turnstile>\<^sub>t\<^sub>y \<tau> : \<star>"
+proof (induction \<Gamma> \<Delta> e \<tau> rule: Tm.induct)
+  case (Tm_Var \<Delta> \<Gamma> x \<tau>)
+  then obtain \<Gamma>1 \<Gamma>2 where 1: "\<Gamma> = \<Gamma>1 @ BVar x \<tau> # \<Gamma>2" using isin_split by blast
+  then have "\<Gamma>2 , \<Delta> \<turnstile>\<^sub>t\<^sub>y \<tau> : \<star>" using context_regularity Tm_Var(1) by blast
+  then show ?case using weaken_ty[of "[]" \<Gamma>2 \<Delta> \<tau> \<star> "\<Gamma>1 @ [BVar x \<tau>]"] Tm_Var(1) 1 by simp
+next
+  case (Tm_Abs x \<tau>1 \<Gamma> \<Delta> e \<tau>2)
+  have 1: "\<Gamma> , \<Delta> \<turnstile>\<^sub>t\<^sub>y \<tau>1 : \<star>" using context_regularity context_valid(1)[OF Tm_Abs(2)] by blast
+  have 2: "\<Gamma> , \<Delta> \<turnstile>\<^sub>t\<^sub>y \<tau>2 : \<star>" using strengthen(2)[of "[]"] Tm_Abs(2) by force
+  have 3: "\<Delta> \<turnstile> \<Gamma>" by (rule context_valid(1)[OF 1])
+  show ?case by (rule Ty_App[OF Ty_App[OF Ty_Arrow[OF 3] 1] 2])
+next
+  case (Tm_TApp \<Gamma> \<Delta> e a k \<sigma> \<tau>)
+  obtain a' \<sigma>' where P: "(\<forall> a:k. \<sigma>) = (\<forall> a':k. \<sigma>')" "BTyVar a' k # \<Gamma> , \<Delta> \<turnstile>\<^sub>t\<^sub>y \<sigma>' : \<star>" by (cases rule: Ty.cases[OF Tm_TApp(3)]) auto
+  have "\<Gamma> , \<Delta> \<turnstile>\<^sub>t\<^sub>y \<sigma>'[\<tau>/a'] : \<star>" using type_substitution_ty[of "[]", OF _ Tm_TApp(2)] P by auto
+  then show ?case using P(1) subst_type_same by auto
+next
+  case (Tm_Ctor \<Delta> \<Gamma> D \<tau>)
+  from Tm_Ctor(1) have 1: "\<turnstile> \<Delta>" by (rule axioms_valid(1))
+  then obtain \<Delta>1 \<Delta>2 where 2: "\<Delta> = \<Delta>1 @ AxCtor D \<tau> # \<Delta>2" using axiom_isin_split[OF Tm_Ctor(2) 1] by blast
+  then have "[] , \<Delta>2 \<turnstile>\<^sub>t\<^sub>y \<tau> : \<star>" using axioms_regularity 1 by blast
+  then have "[] , \<Delta> \<turnstile>\<^sub>t\<^sub>y \<tau> : \<star>" using weaken(3)[of "[]" "[]" \<Delta>2 \<tau> \<star> "\<Delta>1 @ [AxCtor D \<tau>]"] 1 2 Ctx_Empty by simp
+  then show ?case using weaken(2)[of "[]" "[]"] Tm_Ctor(1) by simp
+next
+  case (Tm_Let \<Gamma> \<Delta> e1 \<tau>1 x e2 \<tau>2)
+  then show ?case using strengthen(2)[of "[]"] by force
+qed (auto intro: Ty_intros)
+
+lemma axioms_cons_valid[elim]: "\<turnstile> ax # \<Delta> \<Longrightarrow> (\<turnstile> \<Delta> \<Longrightarrow> P) \<Longrightarrow> P"
+  by (cases rule: Ax.cases) (auto simp: axioms_valid(2))
+
+lemma supp_in_context_ty: "\<Gamma> , \<Delta> \<turnstile>\<^sub>t\<^sub>y \<tau> : k \<Longrightarrow> supp \<tau> \<subseteq> supp \<Gamma>"
+proof (induction \<Gamma> \<Delta> \<tau> k rule: Ty_induct)
+  case (Var \<Gamma> \<Delta> a k)
+  then show ?case by (metis \<tau>.supp(1) fresh_def fresh_not_isin_tyvar singletonD subsetCI supp_at_base)
+next
+  case (Forall \<Gamma> \<Delta> a k \<sigma>)
+  from Forall(2) show ?case unfolding supp_Cons binder.supp(2) \<tau>.supp(5) pure_supp supp_at_base by auto
+qed (auto simp: \<tau>.supp pure_supp)
+
+lemma axioms_empty_supp: "\<turnstile> \<Delta> \<Longrightarrow> supp \<Delta> = {}"
+proof (induction \<Delta>)
+  case (Cons a \<Delta>)
+  then show ?case
+  proof (cases a rule: axiom.exhaust)
+    case (AxData D k)
+    then have "supp \<Delta> = {}" using Cons by blast
+    then show ?thesis using AxData pure_supp axiom.supp(1) unfolding supp_Cons by auto
+  next
+    case (AxCtor K \<tau>)
+    then have "[] , \<Delta> \<turnstile>\<^sub>t\<^sub>y \<tau> : \<star>" using Cons by blast
+    then have 1: "supp \<tau> = {}" using supp_in_context_ty supp_Nil by blast
+    have 2: "supp \<Delta> = {}" using Cons by auto
+    then show ?thesis using 1 AxCtor axiom.supp(2) pure_supp unfolding supp_Cons by blast
+  qed
+qed (simp add: supp_Nil)
+
+corollary permute_axioms[simp]: "\<turnstile> \<Delta> \<Longrightarrow> p \<bullet> \<Delta> = \<Delta>"
+  using axioms_empty_supp by (simp add: fresh_star_def supp_perm_eq)
+
+corollary supp_cty: "\<lbrakk> \<turnstile> \<Delta> ; AxCtor K cty \<in> set \<Delta> \<rbrakk> \<Longrightarrow> supp cty = {}"
+  using axioms_empty_supp by (metis axiom.supp(2) axioms_split_valid split_list sup_bot.neutr_eq_iff supp_Cons)
+
+lemma supp_args:
+  assumes "\<Gamma> , \<Delta> \<turnstile> e : \<tau>1" "head_data \<tau>1 = Some (T, \<sigma>s)" "AxCtor K cty \<in> set \<Delta>" "subst_ctor cty \<sigma>s = Some args"
+  shows "supp args \<subseteq> supp \<Gamma>"
+proof -
+  have 1: "supp cty = {}" by (rule supp_cty[OF axioms_valid(3)[OF assms(1)] assms(3)])
+  have "\<Gamma> , \<Delta> \<turnstile>\<^sub>t\<^sub>y \<tau>1 : \<star>" by (rule typing_regularity[OF assms(1)])
+  then have "supp \<tau>1 \<subseteq> supp \<Gamma>" by (rule supp_in_context_ty)
+  then have "supp \<sigma>s \<subseteq> supp \<Gamma>" using supp_head_data[OF assms(2)] by simp
+  then show "supp args \<subseteq> supp \<Gamma>" using supp_subst_ctor[OF assms(4)] 1 by simp
+qed
+
+lemma supp_in_context_term: "\<Gamma> , \<Delta> \<turnstile> e : \<tau> \<Longrightarrow> supp e \<subseteq> supp \<Gamma>"
+proof (induction \<Gamma> \<Delta> e \<tau> rule: Tm.induct)
+case (Tm_Var \<Delta> \<Gamma> x \<tau>)
+  then show ?case sorry
+next
+  case (Tm_Abs x \<tau>1 \<Gamma> \<Delta> e \<tau>2)
+  then show ?case sorry
+next
+  case (Tm_App \<Gamma> \<Delta> e1 \<tau>1 \<tau>2 e2)
+  then show ?case sorry
+next
+  case (Tm_TAbs a k \<Gamma> \<Delta> e \<sigma>)
+  then show ?case sorry
+next
+  case (Tm_TApp \<Gamma> \<Delta> e a k \<sigma> \<tau>)
+  then show ?case sorry
+next
+  case (Tm_Ctor \<Delta> \<Gamma> D \<tau>)
+  then show ?case sorry
+next
+  case (Tm_Let \<Gamma> \<Delta> e1 \<tau>1 x e2 \<tau>2)
+  then show ?case sorry
+next
+  case (Tm_Case \<Gamma> \<Delta> e \<tau>1 T \<sigma>s \<tau> alts)
+  have "\<forall>alt |\<in>| set_alts alts. supp alt \<subseteq> supp \<Gamma>" using Tm_Case(6)
+  proof (induction rule: alts_induct)
+    case (MatchCtor K tys vals e' cty ks args)
+    have "supp args \<subseteq> supp \<Gamma>" by (rule supp_args[OF Tm_Case(1,2) MatchCtor(1,3)])
+    then have "supp e' \<subseteq> supp tys \<union> supp vals \<union> supp \<Gamma>" using supp_zip_with MatchCtor(5) unfolding supp_append by fastforce
+    then show ?case unfolding alt_supp pure_supp using supp_vars supp_tyvars by auto
+  qed
+  then have "supp alts \<subseteq> supp \<Gamma>"
+    by (induction alts rule: term_alt_list_alt.inducts(2)) (auto simp: alt_list_supp)
+  then show ?case using Tm_Case term_supp by auto
+qed
 
 lemma fresh_in_context_term_var: "\<lbrakk> \<Gamma> , \<Delta> \<turnstile> e : \<tau> ; atom (y::var) \<sharp> \<Gamma> \<rbrakk> \<Longrightarrow> atom y \<sharp> e"
 proof (induction \<Gamma> \<Delta> e \<tau> rule: Tm.induct)
